Compiler/Proofs/YulGeneration/Builtins.lean
@@ -102,6 +102,14 @@ def evalBuiltinCall
     match argVals with
     | [] => some sender
     | _ => none
+  else if func = "callvalue" then
+    match argVals with
+    | [] => some 0
+    | _ => none
+  else if func = "calldatasize" then
+    match argVals with
+    | [] => some (4 + calldata.length * 32)
+    | _ => none
   else if func = "calldataload" then
     match argVals with
     | [offset] => some (calldataloadWord selector calldata offset)
