Compiler/Proofs/TempCounter.lean
@@ -1,0 +1,7 @@
+import Compiler.Proofs.YulGeneration.Equivalence
+
+open Compiler
+open Compiler.Proofs.IRGeneration
+open Compiler.Proofs.YulGeneration
+
+#eval (1+1)
